src/lib/sparse/Kuiper.Sparse.Load.fst
@@ -7,42 +7,41 @@ open Kuiper.Sparse
 open Kuiper.Array.Vectorized
 open Kuiper.Array2.Vectorized
 open Kuiper.EMatrix
+open Kuiper.Tensor
 open Kuiper.Tensor.Layout.Alg { l2_row_major }
-open Kuiper.Array2.Strided { strided_row_major, cell_of_pos }
+open Kuiper.Array2.Strided
 module T = Kuiper.Tensor
-module A = Kuiper.Array1
-module M = Kuiper.Array2
 module SZ = Kuiper.SizeT
 
 
 inline_for_extraction noextract
-fn gpu_load_cell
+fn load_cell
   (#et : Type0)
   (#m #n : sz)
-  (x : gpu_array et m)
+  (x : larray et m)
   (i : szlt m)
-  (y : gpu_array et n)
+  (y : larray et n)
   (#f : perm)
   (#s : erased (lseq et n))
   (j : szlt n)
   preserves gpu ** y |-> Frac f s
   requires array_live_cell x i
-  ensures  gpu_pts_to_cell x i (s @! j)
+  ensures  Cell (x <: array et) (SZ.v i) |-> Seq.index s j
 {
   unfold array_live_cell x;
-  gpu_array_write x i (gpu_array_read y j);
-  with t. assert gpu_pts_to_slice x i (i + 1) t;
-  assert pure (Seq.equal t seq![s @! j]);
+  slice_write x i (Pulse.Lib.Array.(y.(j)));
+  with t. assert pts_to_slice x i (i + 1) t;
+  assert pure (Seq.equal t seq![Seq.index s j]);
 }
 
 inline_for_extraction noextract
-fn gpu_array_vec_cpy_device
+fn array_vec_cpy_device
   (#a : Type u#0) {| sized a, has_vec_cpy a |}
   (#dsz : erased nat)
-  (d : gpu_array a dsz) (doff : sz)
+  (d : larray a dsz) (doff : sz)
   (#_ : squash (aligned' 16 d doff))
   (#ssz : erased nat)
-  (s : gpu_array a ssz) (soff : sz)
+  (s : larray a ssz) (soff : sz)
   (#_ : squash (aligned' 16 s soff))
   (#i #j : erased nat)
   (#f : perm)
@@ -50,40 +49,41 @@ fn gpu_array_vec_cpy_device
   (#_ : squash (i <= soff /\ soff <= j - chunk a))
   (#_ : squash (len v == j - i))
   preserves gpu
-  preserves gpu_pts_to_slice s #f i j v
-  requires gpu_live_vec d doff
+  preserves pts_to_slice s #f i j v
+  requires live_vec d doff
   requires pure (aligned' 16 s soff)
-  ensures  gpu_pts_to_vec' d doff v (soff - i)
+  ensures  pts_to_vec' d doff v (soff - i)
 {
-  unfold gpu_live_vec d;
-  with u_. assert gpu_pts_to_vec d doff u_;
-  gpu_pts_to_slice_ref d doff (doff + chunk a);
-  gpu_pts_to_slice_ref s i j;
-  gpu_array_vec_cpy_dd d doff s soff;
-  with u. assert gpu_pts_to_vec d doff u;
+  unfold live_vec d;
+  with u_. assert pts_to_vec d doff u_;
+  pts_to_slice_ref d doff (doff + chunk a);
+  pts_to_slice_ref s i j;
+  array_vec_cpy d doff s soff;
+  with u. assert pts_to_vec d doff u;
   assert pure (u `Seq.equal` Seq.slice v (soff - i) (soff - i + chunk a));
 }
 
 inline_for_extraction noextract
-fn gpu_array_vec_cpy_local
+fn array_vec_cpy_local
   (#a : Type u#0) {| sized a, has_vec_cpy a |}
   (#dsz : erased nat)
-  (d : gpu_array a dsz) (doff : sz)
+  (d : larray a dsz) (doff : sz)
   (#_ : squash (aligned' 16 d doff))
   (#ssz : erased nat)
   (s : larray a ssz) (soff : sz { soff + chunk a <= ssz})
+  (#_ : squash (aligned' 16 s soff))
   (#f : perm)
   (#v : erased (lseq a ssz))
   preserves gpu
   preserves s |-> Frac f v
-  requires gpu_live_vec d doff
-  ensures  gpu_pts_to_vec' d doff v soff
+  requires live_vec d doff
+  ensures  pts_to_vec' d doff v soff
 {
-  unfold gpu_live_vec d;
-  with u_. assert gpu_pts_to_vec d doff u_;
-  gpu_pts_to_slice_ref d doff (doff + chunk a);
-  gpu_array_vec_cpy_hd d doff s soff;
-  with u. assert gpu_pts_to_vec d doff u;
+  unfold live_vec d;
+  with u_. assert pts_to_vec d doff u_;
+  pts_to_slice_ref d doff (doff + chunk a);
+  array_vec_cpy d doff s soff;
+  with u. assert pts_to_vec d doff u;
   assert pure (u `Seq.equal` Seq.slice v soff (soff + chunk a));
 }
 
@@ -91,8 +91,8 @@ inline_for_extraction noextract
 fn matrix_vec_store
   (#et:Type0) {| sized et, has_vec_cpy et |}
   (#rows #cols : erased nat)
-  (#l : M.layout rows cols) {| T.ctlayout l, strided : strided_row_major l |}
-  (gm : M.array2 et l)
+  (#l : layout2 rows cols) {| T.ctlayout l, strided : strided_row_major l |}
+  (gm : array2 et l)
   (i : szlt rows)
   (j : sz { j + chunk et <= cols })
   (#n : erased nat)
@@ -102,169 +102,243 @@ fn matrix_vec_store
   (k : sz { k + chunk et <= n })
   preserves gpu
   preserves arr |-> Frac f s
+  requires  pure (aligned' 16 arr k)
   requires  matrix_live_vec gm i j
-  requires  pure (aligned' 16 (M.core gm) (cell_of_pos l i j))
+  requires  pure (aligned' 16 (core gm) (cell_of_pos l i j))
+  requires  pure (aligned_strided_row_major (chunk et) strided)
   ensures   matrix_pts_to_vec_slice gm i j s k
 {
   unfold matrix_live_vec gm;
   with v. assert matrix_pts_to_vec gm i j v;
-  unfold matrix_pts_to_vec gm;
+  unfold matrix_pts_to_vec gm i j _;
 
   strided.pf i j;
   let offset : sz = strided.offset +^ strided.stride *^ i +^ j;
 
   forevery_map #(natlt (chunk et))
-    (fun x -> M.pts_to_cell gm ((SZ.v i <: natlt rows), (j + x)) (v @! x))
-    (fun x -> gpu_pts_to_cell (M.core gm) (offset + x) (v @! x))
+    (fun x -> Cell gm (idx2 (i <: natlt rows) (j + x <: natlt cols)) |-> (Seq.index v x))
+    (fun x -> Cell (core gm <: array et) (offset + x <: nat) |-> (Seq.index v x))
     fn x {
       let j' : natlt cols = j + x;
       assert rewrites_to j' (j + x);
       let i' : natlt rows = SZ.v i;
       assert rewrites_to i' (SZ.v i);
 
-      M.pts_to_cell_eq gm (i', j') 1.0R (v @! x);
+      tensor_pts_to_cell_eq gm (idx2 i' j') 1.0R (Seq.index v x);
       strided.pf i' j';
 
-      rewrite M.pts_to_cell gm (i', j') (v @! x)
-      as gpu_pts_to_cell (M.core gm) (offset + x) (v @! x);
+      rewrite Cell gm (idx2 i' j') |-> Seq.index v x
+      as Cell (core gm <: array et) (offset + x <: nat) |-> Seq.index v x;
     };
 
   forevery_rw_size (chunk et) ((offset + chunk et) - offset);
   strided.pf i (j + chunk et - 1);
-  gpu_array_unslice_1' (M.core gm) offset (offset + chunk et);
-  fold gpu_live_vec (M.core gm) offset;
+  array_unslice_1' (core gm) offset (offset + chunk et);
+  fold live_vec (core gm) offset;
 
-  gpu_array_vec_cpy_local (M.core gm) offset arr k;
+  array_vec_cpy_local (core gm) offset arr k;
 
-  gpu_array_slice_1' (M.core gm) offset (offset + chunk et);
+  array_slice_1' (core gm) offset (offset + chunk et);
   forevery_rw_size ((offset + chunk et) - offset) (chunk et);
   forevery_map #(natlt (chunk et))
-    (fun x -> gpu_pts_to_cell (M.core gm) (offset + x) (Seq.slice s k (k + chunk et) @! x))
-    (fun x -> M.pts_to_cell gm ((SZ.v i <: natlt rows), (j + x)) (seq_chunk s k @! x))
+    (fun x ->
+      pts_to_cell
+        (core gm)
+        (offset + x)
+        (Seq.index (Seq.slice s k (k + chunk et)) x)
+    )
+    (fun x ->
+      tensor_pts_to_cell gm (idx2 i (j + x)) (Seq.index (seq_chunk s k) x)
+    )
     fn x {
       let j' : natlt cols = j + x;
       assert rewrites_to j' (j + x);
       let i' : natlt rows = SZ.v i;
       assert rewrites_to i' (SZ.v i);
 
-      M.pts_to_cell_eq gm (i', j') 1.0R (Seq.slice s k (k + chunk et) @! x);
+      tensor_pts_to_cell_eq gm (idx2 i' j') 1.0R (Seq.index (Seq.slice s k (k + chunk et)) x);
       strided.pf i' j';
 
-      assert pure (Seq.slice s k (k + chunk et) @! x == seq_chunk s k @! x);
-      rewrite gpu_pts_to_cell (M.core gm) (offset + x) (Seq.slice s k (k + chunk et) @! x)
-      as M.pts_to_cell gm (i', j') (seq_chunk s k @! x);
+      // assert pure (Seq.slice s k (k + chunk et) @! x == seq_chunk s k @! x);
+      rewrite
+        pts_to_cell
+          (core gm)
+          (offset + x)
+          (Seq.index (Seq.slice s k (k + chunk et)) x)
+      as tensor_pts_to_cell gm (idx2 i' j') (Seq.index (seq_chunk s k) x);
     };
   fold matrix_pts_to_vec gm i j (seq_chunk s k);
   fold matrix_pts_to_vec_slice gm i j s k;
 }
 
-open Kuiper.Seq.Common { seq_blit }
-let seq_blit'
+// TODO  mover estas definiciones
+let chest_blit
   (#a:Type)
   (#n1 : nat)
-  (s1 : lseq a n1) (off1 : natlt n1)
+  (s1 : chest1 a n1) (off1 : nat)
   (#n2 : nat)
-  (s2 : lseq a n2) (off2 : nat)
+  (s2 : chest1 a n2) (off2 : nat)
+  (cnt : nat{off1 + cnt <= n1 /\ off2 + cnt <= n2})
+  : chest1 a n1
+=
+  mk1 fun i ->
+    if i < off1 || off1 + cnt <= i
+      then acc1 s1 i
+      else acc1 s2 (off2 + i - off1)
+
+let chest1_blit'
+  (#a:Type)
+  (#n1 : nat)
+  (s1 : chest1 a n1) (off1 : natlt n1)
+  (#n2 : nat)
+  (s2 : chest1 a n2) (off2 : nat)
   (cnt : nat { cnt /? n1 /\ cnt /? off1 /\ cnt /? n2 /\ cnt /? off2 } )
-  : lseq a n1
+  : chest1 a n1
 =
   lemma_divides_leq cnt n1 off1;
   lemma_divides_leq cnt n2 off2;
   if off2 < n2
-    then seq_blit s1 off1 s2 off2 cnt
+    then chest_blit s1 off1 s2 off2 cnt
     else s1
 
+open Kuiper.Shape { abs_bring_forward_bij }
+open Kuiper.Bijection
+
+let prod_unit_bij (a : Type) : (a & unit =~ a) =
+{
+  ff = (fun (x, ()) -> x);
+  gg = (fun x -> (x, ()));
+
+  ff_gg = ez;
+  gg_ff = ez;
+}
+
+ghost
+fn forevery_abs1_iso
+  (#n : nat)
+  (p : abs (n @| INil) -> slprop)
+  requires forall+ (i : abs (n @| INil)). p i
+  ensures  forall+ (i : natlt n). p (idx1 i)
+{
+  forevery_iso (abs_bring_forward_bij 0 (n @| INil)) _;
+  rewrite each ((n @| INil) @! 0) as n;
+  rewrite each abs (modulo_i 0 (n @| INil)) as unit;
+  forevery_iso (prod_unit_bij (natlt n)) _;
+  forevery_ext _ (fun i -> p (idx1 i));
+}
+
+ghost
+fn forevery_abs1_iso_back
+  (#n : nat)
+  (p : abs (n @| INil) -> slprop)
+  requires forall+ (i : natlt n). p (idx1 i)
+  ensures  forall+ (i : abs (n @| INil)). p i
+{
+  forevery_iso (bij_sym (prod_unit_bij (natlt n))) _;
+  rewrite each n as ((n @| INil) @! 0);
+  rewrite each unit as abs (modulo_i 0 (n @| INil));
+  forevery_iso (bij_sym (abs_bring_forward_bij 0 (n @| INil))) _;
+  forevery_ext _ p;
+}
 
 ghost
 fn lower_cont
   (#et : Type u#0)
   (#sz : pos)
-  (#l : A.layout sz) {| cl : cont_layout l |}
-  (a : A.array1 et l)
+  (#l : layout1 sz) {| cl : cont_layout l |}
+  (a : array1 et l)
   (#f : perm)
-  (#s : lseq et sz)
+  (#s : chest1 et sz)
   requires a |-> Frac f s
-  ensures  gpu_pts_to_slice (A.core a) #f cl.offset (cl. offset + sz) s
+  ensures  pts_to_slice (core a) #f cl.offset (cl. offset + sz) (chest1_to_seq s)
 {
-  A.explode a;
+  tensor_explode a;
+  let s' = chest1_to_seq s;
+
+  forevery_abs1_iso _;
+
   forevery_map #(natlt sz)
-    (fun i -> Cell a i |-> Frac f (s @! i))
-    (fun i -> Cell (A.core a) (cl.offset + i <: nat) |-> Frac f (s @! i))
+    (fun i -> Cell a (idx1 i) |-> Frac f (acc s (idx1 i)))
+    (fun i -> Cell (core a <: array et) (cl.offset + i <: nat) |-> Frac f (Seq.index s' i))
     fn i {
       cl.pf i;
-      A.pts_to_cell_eq a i f (s @! i);
-      rewrite  Cell a i |-> Frac f (s @! i)
-      as Cell (A.core a) (cl.offset + i <: nat) |-> Frac f (s @! i);
+      tensor_pts_to_cell_eq a (idx1 i) f (acc s (idx1 i));
+      rewrite  Cell a (idx1 i) |-> Frac f (acc s (idx1 i))
+      as pts_to_cell (core a) #f (cl.offset + i) (Seq.index s' i);
     };
   cl.pf (sz - 1);
   forevery_rw_size sz ((cl.offset + sz) - cl.offset);
-  gpu_array_unslice_1' (A.core a) cl.offset (cl.offset + sz);
+  array_unslice_1' (core a) cl.offset (cl.offset + sz);
 }
 
 ghost
 fn raise_cont
   (#et : Type u#0)
   (#sz : pos)
-  (#l : A.layout sz) {| cl : cont_layout l |}
-  (a : A.array1 et l)
+  (#l : layout1 sz) {| cl : cont_layout l |}
+  (a : array1 et l)
   (#f : perm)
   (#s : lseq et sz)
-  requires pure (fits (A.layout_size l))
-  requires gpu_pts_to_slice (A.core a) #f cl.offset (cl. offset + sz) s
-  ensures  a |-> Frac f s
+  requires pure (fits (tlayout_ulen l))
+  requires pts_to_slice (core a) #f cl.offset (cl. offset + sz) s
+  ensures  a |-> Frac f (seq_to_chest1 s)
 {
+  let s' = seq_to_chest1 s;
   cl.pf (sz - 1);
-  gpu_array_slice_1' (A.core a) cl.offset (cl.offset + sz);
+  array_slice_1' (core a) cl.offset (cl.offset + sz);
   forevery_rw_size ((cl.offset + sz) - cl.offset) sz;
   forevery_map #(natlt sz)
-    (fun i -> Cell (A.core a) (cl.offset + i <: nat) |-> Frac f (s @! i))
-    (fun i -> Cell a i |-> Frac f (s @! i))
+    (fun i ->
+      Cell (core a <: array et) (cl.offset + i <: nat) |-> Frac f (Seq.index s i))
+    (fun i -> Cell a (idx1 i) |-> Frac f (acc s' (idx1 i)))
     fn i {
       cl.pf i;
-      A.pts_to_cell_eq a i f (s @! i);
-      rewrite Cell (A.core a) (cl.offset + i <: nat) |-> Frac f (s @! i)
-      as  Cell a i |-> Frac f (s @! i);
+      tensor_pts_to_cell_eq a (idx1 i) f (Seq.index s i);
+      rewrite Cell (core a <: array et) (cl.offset + i <: nat) |-> Frac f (Seq.index s i)
+      as  Cell a (idx1 i) |-> Frac f (acc s' (idx1 i));
     };
-  A.implode a;
+  forevery_abs1_iso_back #sz
+    (fun i -> tensor_pts_to_cell a #f i (acc s' i));
+  tensor_implode a;
 }
 
 let aligned_cont_offset
   (#et : Type u#0) {| sized et, has_vec_cpy et |}
   (#sz : erased nat)
-  (#l : A.layout sz) {| cl : cont_layout l |}
-  (a : A.array1 et l)
+  (#l : layout1 sz) {| cl : cont_layout l |}
+  (a : array1 et l)
   (off : erased nat { chunk et /? off })
 : Lemma
   (requires
-    aligned 16 (A.core a) /\
+    aligned 16 (core a) /\
     aligned_cont_layout (chunk et) cl
   )
-  (ensures aligned' 16 (A.core a) (cl.offset + off))
+  (ensures aligned' 16 (core a) (cl.offset + off))
 = ()
 
-#push-options "--split_queries always --z3rlimit 10"
+#push-options "--split_queries always --z3rlimit 15"
 noextract
-fn array_vec_cpy
+fn array_vec_cpy'
   (#et : Type u#0) {| sized et, has_vec_cpy et |}
   (#dst_sz : erased nat { 0 < dst_sz /\ chunk et /? dst_sz })
-  (#dst_l : A.layout dst_sz) {| T.ctlayout dst_l, dst_cl : cont_layout dst_l |}
-  (dst_arr : A.array1 et dst_l)
+  (#dst_l : layout1 dst_sz) {| T.ctlayout dst_l, dst_cl : cont_layout dst_l |}
+  (dst_arr : array1 et dst_l)
   (dst_off : szlt dst_sz { chunk et /? dst_off })
   (#src_sz : szp { chunk et /? src_sz })
-  (#src_l : A.layout src_sz) {| T.ctlayout src_l, src_cl : cont_layout src_l |}
-  (src_arr : A.array1 et src_l)
+  (#src_l : layout1 src_sz) {| T.ctlayout src_l, src_cl : cont_layout src_l |}
+  (src_arr : array1 et src_l)
   (src_off : sz { chunk et /? src_off })
   (#f : perm)
-  (#ds : erased (lseq et dst_sz))
-  (#ss : erased (lseq et src_sz))
+  (#ds : chest1 et dst_sz)
+  (#ss : chest1 et src_sz)
   preserves gpu
   requires  dst_arr |-> ds
-  requires  pure (aligned 16 (A.core dst_arr))
+  requires  pure (aligned 16 (core dst_arr))
   requires  pure (aligned_cont_layout (chunk et) dst_cl)
   preserves src_arr |-> Frac f ss
-  requires  pure (aligned 16 (A.core src_arr))
+  requires  pure (aligned 16 (core src_arr))
   requires  pure (aligned_cont_layout (chunk et) src_cl)
-  ensures   dst_arr |-> seq_blit' ds dst_off ss src_off (chunk et)
+  ensures   dst_arr |-> chest1_blit' ds dst_off ss src_off (chunk et)
 {
   if (src_off <^ src_sz)
   {
@@ -277,34 +351,46 @@ fn array_vec_cpy
     aligned_cont_offset dst_arr (SZ.v dst_off);
     aligned_cont_offset src_arr (SZ.v src_off);
 
-    gpu_array_vec_cpy_dd
-      (A.core dst_arr) (dst_cl.offset +^ dst_off)
-      (A.core src_arr) (src_cl.offset +^ src_off);
+    array_vec_cpy
+      (core dst_arr) (dst_cl.offset +^ dst_off)
+      (core src_arr) (src_cl.offset +^ src_off);
 
     raise_cont dst_arr;
     raise_cont src_arr #f;
+
+    with ds'. assert dst_arr |-> ds';
+    assert pure (
+      ds' `equal` (chest1_blit' ds dst_off ss src_off (chunk et))
+    );
+
+    with ss'. assert src_arr |-> Frac f ss';
+    assert pure (ss' `equal` ss);
   }
   else
   {
-    ();
+    assert pure (
+      ds `equal` (chest1_blit' ds dst_off ss src_off (chunk et))
+    );
   }
 }
 #pop-options
 
+#push-options "--z3rlimit 10"
 noextract
 fn array_vec_cpy_dh
   (#et : Type u#0) {| sized et, has_vec_cpy et |}
   (dst_arr : larray et (chunk et))
   (#src_sz : szp { chunk et /? src_sz })
-  (#src_l : A.layout src_sz) {| T.ctlayout src_l, src_cl : cont_layout src_l |}
-  (src_arr : A.array1 et src_l)
+  (#src_l : layout1 src_sz) {| T.ctlayout src_l, src_cl : cont_layout src_l |}
+  (src_arr : array1 et src_l)
   (src_off : szlt src_sz { chunk et /? src_off })
   (#f : perm)
   (#ss : erased (lseq et src_sz))
   preserves gpu
   requires  live dst_arr
-  preserves src_arr |-> Frac f ss
-  requires  pure (aligned 16 (A.core src_arr))
+  requires  pure (aligned 16 dst_arr)
+  preserves src_arr |-> Frac f (seq_to_chest1 ss)
+  requires  pure (aligned 16 (core src_arr))
   requires  pure (aligned_cont_layout (chunk et) src_cl)
   ensures   dst_arr |-> Seq.slice ss src_off (src_off + chunk et)
 {
@@ -315,12 +401,16 @@ fn array_vec_cpy_dh
     aligned_cont_offset src_arr (SZ.v src_off);
 
     Pulse.Lib.Array.PtsTo.pts_to_len dst_arr;
-    gpu_array_vec_cpy_dh
+    array_vec_cpy
       dst_arr 0sz
-      (A.core src_arr) (src_cl.offset +^ src_off);
+      (core src_arr) (src_cl.offset +^ src_off);
 
     raise_cont src_arr #f;
 
     with s. assert dst_arr |-> s;
     assert pure (Seq.equal s (Seq.slice ss src_off (src_off + chunk et)));
+
+    with ss'. assert src_arr |-> Frac f ss';
+    assert pure (ss' `equal` seq_to_chest1 ss);
 }
+#pop-options
