src/lib/sparse/Kuiper.Sparse.SPMM.Mask.fst
@@ -9,19 +9,19 @@ open Kuiper.Array2.Vectorized
 open Kuiper.EMatrix
 
 inline_for_extraction noextract
-fn gpu_mask_cell
+fn mask_cell
   (#et : Type0)
   (#n : sz)
-  (x : gpu_array et n)
+  (x : larray et n)
   (i : szlt n)
   (z : et)
   preserves gpu
   requires array_live_cell x i
-  ensures  gpu_pts_to_cell x i z
+  ensures  pts_to_cell x i z
 {
   unfold array_live_cell x;
-  gpu_array_write x i z;
-  with s. assert gpu_pts_to_slice x i (i + 1) s;
+  slice_write x i z;
+  with s. assert pts_to_slice x i (i + 1) s;
   assert pure (Seq.equal s seq![z]);
 }
 
@@ -33,7 +33,7 @@ inline_for_extraction noextract
 fn mask_array
   (#et : Type0)
   (#n : sz)
-  (x : gpu_array et n)
+  (x : larray et n)
   (to : szle n)
   (z : et)
   (nthr : sz)
@@ -49,22 +49,19 @@ fn mask_array
   forevery_rw_size ((to - 0 - tid) `divup` nthr) to_;
 
   foreach to_
-    (fun k ->
-      array_live_cell x (0 + k * nthr + tid)
-    )
-    (fun k ->
-      gpu_pts_to_cell x (k * nthr + tid) z
-    )
+    (fun k -> array_live_cell x (0 + k * nthr + tid))
+    (fun k -> Cell (x <: array et) (k * nthr + tid <: nat) |-> z)
     #gpu
     fn k {
       rewrite each (0 + k * nthr + tid) as (k * nthr + tid);
-      gpu_mask_cell x (k *^ nthr +^ tid) z;
+      mask_cell x (k *^ nthr +^ tid) z;
     };
 
   forevery_rw_size to_ ((to - 0 - tid) `divup` nthr);
 
   forevery_ext #(natlt ((to - 0 - tid) `divup` nthr))
-    (fun k -> gpu_pts_to_cell x (k * nthr + tid) z)
-    (fun k -> gpu_pts_to_cell x (0 + k * nthr + tid) z);
+    (fun k -> Cell (x <: array et) (k * nthr + tid <: nat) |-> z)
+    (fun k -> Cell (x <: array et) (0 + k * nthr + tid <: nat) |-> z);
+
   fold thread_slice_pts_to_value x 0 to z nthr tid;
 }
